kuiops/gather/Kuiops.Gather.fsti
@@ -12,47 +12,29 @@ module SZ = Kuiper.SizeT
 let gather_chest 
   (#et : Type0)
   (#r : erased nat)
-  (d : shape r)
-  (eInp : chest d et)
+  (di do : shape r { shape_le di do })
+  (eInp : chest do et)
   (dim : natlt r)
-  (eIdx : chest d (szlt (d @! dim))): chest d et
-  = Kuiper.Chest.mk d
-      (fun (x : abs d) ->
+  (eIdx : chest di (szlt (do @! dim))): chest di et
+  = Kuiper.Chest.mk di
+      (fun (x : abs di) ->
          let idx = acc eIdx x in
-         let x' = abs_set_at dim idx x in
+         let x' = abs_set_at2 di do dim idx x in
          acc eInp x')
-
-(* LATER: technically, idx and out can be smaller than inp. PyTorch says:
-
-'''
-For a 3-D tensor the output is specified by:
-
-out[i][j][k] = input[index[i][j][k]][j][k]  # if dim == 0
-out[i][j][k] = input[i][index[i][j][k]][k]  # if dim == 1
-out[i][j][k] = input[i][j][index[i][j][k]]  # if dim == 2
-
-input and index must have the same number of dimensions. 
-It is also required that index.size(d) <= input.size(d) for all dimensions d != dim. 
-out will have the same shape as index. Note that input and index do not broadcast against each other. 
-When index is empty, we always return an empty output with the same shape without further error checking.
-'''
-
-I read this to mean the i,j,k in the above example has the ranges of the dimensions of index, NOT of input. 
-And `out` inherits the same shape as index. *)
 
 inline_for_extraction noextract
 fn gather_gpu
-  (#et : Type0) (#r : erased nat) (d : shape r) (cd: cshape d)
+  (#et : Type0) (#r : erased nat) (di do : shape r { shape_le di do }) (cdi: cshape di) (cdo: cshape do)
   (dim: szlt r)
-  (#lInp #lIdx #lOut: tlayout d)  {| ctlayout lInp, ctlayout lIdx, ctlayout lOut |}
+  (#lInp: tlayout do) (#lIdx #lOut: tlayout di)  {| ctlayout lInp, ctlayout lIdx, ctlayout lOut |}
   (gInp: tensor et lInp {is_global gInp})
-  (gIdx: tensor (szlt (d @! (SZ.v dim))) lIdx {is_global gIdx})
+  (gIdx: tensor (szlt (do @! (SZ.v dim))) lIdx {is_global gIdx})
   (gOut: tensor et lOut {is_global gOut})
-  (n : sz{SZ.v n == sizeof d /\ n <= max_blocks * max_threads /\ n > 0})
-  (eInp: chest d et)
-  (eIdx: chest d (szlt (d @! (SZ.v dim))))
+  (n : sz{SZ.v n == sizeof di /\ n <= max_blocks * max_threads /\ n > 0})
+  (eInp: chest do et)
+  (eIdx: chest di (szlt (do @! (SZ.v dim))))
   (#fInp #fIdx: perm)
   preserves cpu ** on gpu_loc (gInp |-> Frac fInp eInp) ** on gpu_loc (gIdx |-> Frac fIdx eIdx)
   requires on gpu_loc (live gOut)
   ensures 
-      on gpu_loc (gOut |-> gather_chest d eInp dim eIdx)
+      on gpu_loc (gOut |-> gather_chest di do eInp dim eIdx)
