kuiops/elementwise/Kuiops.Elementwise.fsti
@@ -11,4 +11,7 @@ inline_for_extraction noextract
 let neg (#t:Type0) {| floating t |} (x : t) : t = sub zero x
 
 inline_for_extraction noextract
-let square (#t:Type0) {| floating t |} (x : t) : t = x `mul` x
+let square (#t:Type0) {| scalar t |} (x : t) : t = x `mul` x
+
+inline_for_extraction noextract
+let add_alpha (#t:Type0) {| scalar t |} (x : t) (alpha: t) (y: t): t = x `add` (alpha `mul` y)
