kuiops/gather/Kuiops.Gather.fst
@@ -13,61 +13,61 @@ open Kuiper.Kernel.TMap
 
 module SZ = Kuiper.SizeT
 
-let vfgather (#et: Type0) (#r : erased nat) (d : shape r) (dim : natlt r)
-  (eInp : chest d et) (eIdx : chest d (szlt (d @! dim)))
-  (x : abs d) (_: et) (o: et)
+let vfgather (#et: Type0) (#r : erased nat) (di do : shape r { shape_le di do }) (dim : natlt r)
+  (eInp : chest do et) (eIdx : chest di (szlt (do @! dim)))
+  (x : abs di) (_: et) (o: et)
   : prop 
-  = o == acc eInp (abs_set_at dim (acc eIdx x) x)
+  = o == acc eInp (abs_set_at2 di do dim (acc eIdx x) x)
 
 unfold
-let gather_frame (#et : Type0) (#r : erased nat) (d : shape r) (cd: cshape d)
+let gather_frame (#et : Type0) (#r : erased nat) (di do : shape r { shape_le di do }) (cdi: cshape di)
   (dim: szlt r)
-  (#lInp #lIdx: tlayout d)  {| ctlayout lInp, ctlayout lIdx |}
+  (#lInp: tlayout do) (#lIdx: tlayout di)  {| ctlayout lInp, ctlayout lIdx |}
   (gInp: tensor et lInp {is_global gInp})
-  (gIdx: tensor (szlt (d @! (SZ.v dim))) lIdx {is_global gIdx})
-  (eInp: chest d et)
-  (eIdx: chest d (szlt (d @! (SZ.v dim))))
+  (gIdx: tensor (szlt (do @! (SZ.v dim))) lIdx {is_global gIdx})
+  (eInp: chest do et)
+  (eIdx: chest di (szlt (do @! (SZ.v dim))))
   (fInp fIdx: perm)
   (fr: perm): slprop =
     (tensor_pts_to gInp #((fInp /. (fInp +. fIdx)) *. fr) eInp) **
     (tensor_pts_to gIdx #((fIdx /. (fInp +. fIdx)) *. fr) eIdx) 
 
 instance gather_frame_shareable
-  (#et : Type0) (#r : erased nat) (d : shape r) (cd: cshape d)
+  (#et : Type0) (#r : erased nat) (di do : shape r { shape_le di do }) (cdi: cshape di)
   (dim: szlt r)
-  (#lInp #lIdx: tlayout d)  {| ctlayout lInp, ctlayout lIdx|}
+  (#lInp: tlayout do) (#lIdx: tlayout di)  {| ctlayout lInp, ctlayout lIdx|}
   (gInp: tensor et lInp {is_global gInp})
-  (gIdx: tensor (szlt (d @! (SZ.v dim))) lIdx {is_global gIdx})
-  (eInp: chest d et)
-  (eIdx: chest d (szlt (d @! (SZ.v dim))))
+  (gIdx: tensor (szlt (do @! (SZ.v dim))) lIdx {is_global gIdx})
+  (eInp: chest do et)
+  (eIdx: chest di (szlt (do @! (SZ.v dim))))
   (fInp fIdx: perm):
-  shareable (gather_frame d cd dim #lInp #lIdx gInp gIdx eInp eIdx fInp fIdx) =
+  shareable (gather_frame di do cdi dim #lInp #lIdx gInp gIdx eInp eIdx fInp fIdx) =
     double_shareable 
     (fun fr -> tensor_pts_to gInp #fr eInp) 
     (fun fr -> tensor_pts_to gIdx #fr eIdx)
     (fInp /. (fInp +. fIdx)) (fIdx /. (fInp +. fIdx))
 
 inline_for_extraction noextract
-fn fgather (#et : Type0) (#r : erased nat) (d : shape r) (cd: cshape d)
+fn fgather (#et : Type0) (#r : erased nat) (di do : shape r { shape_le di do }) (cdi: cshape di) (cdo: cshape do)
   (dim: szlt r)
-  (#lInp #lIdx #lOut: tlayout d)  {| ctlayout lInp, ctlayout lIdx, ctlayout lOut |}
+  (#lInp: tlayout do) (#lIdx #lOut: tlayout di)  {| ctlayout lInp, ctlayout lIdx, ctlayout lOut |}
   (gInp: tensor et lInp {is_global gInp})
-  (gIdx: tensor (szlt (d @! (SZ.v dim))) lIdx {is_global gIdx})
+  (gIdx: tensor (szlt (do @! (SZ.v dim))) lIdx {is_global gIdx})
   (gOut: tensor et lOut {is_global gOut})
-  (eInp: chest d et)
-  (eIdx: chest d (szlt (d @! (SZ.v dim))))
+  (eInp: chest do et)
+  (eIdx: chest di (szlt (do @! (SZ.v dim))))
   (#fInp #fIdx: perm)
-  (#fr: perm) (i: conc d) (x : et) 
+  (#fr: perm) (i: conc di) (x : et) 
 norewrite
 preserves
-  (gather_frame d cd dim #lInp #lIdx gInp gIdx eInp eIdx fInp fIdx fr)
+  (gather_frame di do cdi dim #lInp #lIdx gInp gIdx eInp eIdx fInp fIdx fr)
 returns 
   r: et
 ensures
-  pure (vfgather d dim eInp eIdx (up i) x r)
+  pure (vfgather di do dim eInp eIdx (up i) x r)
 {
   let idx = tensor_read gIdx i;
-  let idx' = conc_set_at dim idx i;
+  let idx' = conc_set_at2 cdi cdo dim idx i;
   let inp = tensor_read gInp idx';
 
   return inp;
@@ -75,29 +75,28 @@ ensures
 
 inline_for_extraction noextract
 fn gather_gpu
-  (#et : Type0) (#r : erased nat) (d : shape r) (cd: cshape d)
+  (#et : Type0) (#r : erased nat) (di do : shape r { shape_le di do }) (cdi: cshape di) (cdo: cshape do)
   (dim: szlt r)
-  (#lInp #lIdx #lOut: tlayout d)  {| ctlayout lInp, ctlayout lIdx, ctlayout lOut |}
+  (#lInp: tlayout do) (#lIdx #lOut: tlayout di)  {| ctlayout lInp, ctlayout lIdx, ctlayout lOut |}
   (gInp: tensor et lInp {is_global gInp})
-  (gIdx: tensor (szlt (d @! (SZ.v dim))) lIdx {is_global gIdx})
+  (gIdx: tensor (szlt (do @! (SZ.v dim))) lIdx {is_global gIdx})
   (gOut: tensor et lOut {is_global gOut})
-  (n : sz{SZ.v n == sizeof d /\ n <= max_blocks * max_threads /\ n > 0})
-  (eInp: chest d et)
-  (eIdx: chest d (szlt (d @! (SZ.v dim))))
+  (n : sz{SZ.v n == sizeof di /\ n <= max_blocks * max_threads /\ n > 0})
+  (eInp: chest do et)
+  (eIdx: chest di (szlt (do @! (SZ.v dim))))
   (#fInp #fIdx: perm)
   preserves cpu ** on gpu_loc (gInp |-> Frac fInp eInp) ** on gpu_loc (gIdx |-> Frac fIdx eIdx)
   requires on gpu_loc (live gOut)
   ensures 
-      on gpu_loc (gOut |-> gather_chest d eInp dim eIdx) {
+      on gpu_loc (gOut |-> gather_chest di do eInp dim eIdx) {
   with eOut. assert on gpu_loc (gOut |-> eOut);
-  let kfun = (kmap cd
-      (gather_frame d cd dim #lInp #lIdx gInp gIdx eInp eIdx fInp fIdx)
-      #(gather_frame_shareable d cd dim #lInp #lIdx gInp gIdx eInp eIdx fInp fIdx)
-      (vfgather d dim eInp eIdx) 
-      (fgather d cd dim #lInp #lIdx #lOut gInp gIdx gOut eInp eIdx #fInp #fIdx)
+  launch_sync
+    (kmap cdi
+      (gather_frame di do cdi dim #lInp #lIdx gInp gIdx eInp eIdx fInp fIdx)
+      #(gather_frame_shareable di do cdi dim #lInp #lIdx gInp gIdx eInp eIdx fInp fIdx)
+      (vfgather di do dim eInp eIdx) 
+      (fgather di do cdi cdo dim #lInp #lIdx #lOut gInp gIdx gOut eInp eIdx #fInp #fIdx)
       n gOut #eOut #_ #(fInp +. fIdx));
-  launch_sync 
-    kfun;
   with eOut'. assert on gpu_loc (gOut |-> eOut');
-  assert pure (Kuiper.Chest.equal eOut' (gather_chest d eInp dim eIdx)); 
+  assert pure (Kuiper.Chest.equal eOut' (gather_chest di do eInp dim eIdx)); 
 }
